left bne case

coqimp/framework/logic/logic.v
@@ -321,7 +321,7 @@ Inductive wf_seq : funspec -> asrt -> InsSeq -> asrt -> Prop :=
 | call_rule : forall f f1 f2 i I p p1 p2 p' q r fp fq (L : list logicvar) v (Spec : funspec),
     Spec (f, f +ᵢ ($ 4)) = Some (fp, fq) ->
     (p ↓) ==> r15 |=> v ** p1 ->
-    |- {{ (r15 |=> f1 ** p1) ↓ }} i {{ p2 }} -> p2 ==> ((Or r15) ==ₑ f1) ->
+    |- {{ (r15 |=> f1 ** p1) ↓ }} i {{ p2 }} -> fp L ==> ((Or r15) ==ₑ f1) ->
     p2 ==> fp L ** r -> fq L ** r ==> p'-> fq L ==> ((Or r15) ==ₑ f1) ->
     DlyFrameFree r -> wf_seq Spec p' I q ->
     wf_seq Spec p (f1 c> call f ;; f2 c> i ;; I) q
