coqimp/framework/soundness/wf_seq_sound.v
@@ -6,7 +6,7 @@ Require Import Integers.
 Open Scope Z_scope.    
 Import ListNotations.
   
-Set Asymmetric Patterns. 
+Set Asymmetric Patterns.  
       
 Require Import state.    
 Require Import language. 
@@ -36,6 +36,22 @@ Proof.
   intros.
   inversion H; subst.
   inversion H8; subst; eauto.
+Qed.
+
+(*+ Lemmas for Sep Star +*)
+Lemma sep_star_subst :
+  forall p1 p1' p2 s,
+    s |= p1 ** p2 -> p1 ==> p1' ->
+    s |= p1' ** p2.
+Proof.
+  intros.
+  sep_star_split_tac.
+  simpls.
+  simpljoin1.
+  eapply H0 in H.
+  exists (m, (r, f0), d0) (m0, (r0, f0), d0).
+  simpl.
+  repeat (split; eauto).
 Qed.
 
 (*+ Lemmas for exe-delay +*)
@@ -71,6 +87,66 @@ Proof.
       symmetry in Heqe.
       eapply IHD in Heqe; eauto.
     }
+Qed.
+
+Lemma regz_exe_delay_stable2 :
+  forall D D' (R R' : RegFile) v,
+    R' z = Some v -> (R', D') = exe_delay R D ->
+    R z = Some v.
+Proof.
+  intro D.
+  induction D; intros.
+  -
+    simpls.
+    inversion H0; subst.
+    eauto.
+
+  -
+    destruct a, p.
+    simpls.
+    destruct d.
+    {
+      destruct (exe_delay R D) eqn:Heqe.
+      inversion H0; subst.
+      symmetry in Heqe.
+      eapply IHD in Heqe; eauto.
+      clear - H.
+      unfolds set_R.
+      unfold is_indom in *.
+      destruct (r s) eqn : Heqe; tryfalse; eauto.
+      unfolds RegMap.set.
+      destruct_rneq_H.
+    }
+    {
+      destruct (exe_delay R D) eqn:Heqe.
+      inversion H0; subst.
+      symmetry in Heqe.
+      eapply IHD in Heqe; eauto.
+    }
+Qed.
+
+(*+ Lemmas for register state +*)
+Lemma reg_vl_change :
+  forall M R F D rn v v1 p,
+    (M, (R, F), D) |= rn |=> v ** p ->
+    (M, (set_R R rn v1, F), D) |= rn |=> v1 ** p.
+Proof.
+  intros.
+  sep_star_split_tac.
+  simpls.
+  unfolds regSt.
+  simpls.
+  simpljoin1.
+  exists (empM, (set_R (RegMap.set rn (Some v) empR) rn v1, f0), d0)
+    (m0, (r0, f0), d0).
+  simpl.
+  repeat (split; eauto).
+  eapply disjoint_setR_still1; eauto.
+  rewrite indom_setR_merge_eq1; eauto.
+  eapply regset_l_l_indom; eauto.
+  rewrite indom_setR_eq_RegMap_set; eauto.
+  rewrite regset_twice; eauto.
+  eapply regset_l_l_indom; eauto.
 Qed.
     
 (*+ Lemmas for Safety Instruction Sequence +*)
@@ -288,13 +364,1240 @@ Proof.
       simpl; eauto.
       simpl; eauto.
     }
-    {
+    { 
       intros.
-      
+      simpljoin1.
+      lets Hp : H6.  
+      eapply H7 with (S1 := x) in Hp; eauto.
+      simpljoin1.
+      renames x5 to fp, x6 to fq, x7 to L, x8 to r'.
+      eapply program_step_safety_property with
+      (s := (m1 ⊎ m0, (r1 ⊎ r0, f0), d0)) (r := r) in H6;
+        eauto.
+      simpljoin1.
+      destruct_state x.
+      destruct_state x6.
+      simpl in H16.
+      simpljoin1.
+      eapply program_step_safety_property with
+      (s := (m ⊎ m2, (r2 ⊎ r3, f1), d1)) (r := r) in H11;
+        eauto.
+      simpljoin1.
+      destruct_state x0.
+      destruct_state x5.
+      simpl in H19.
+      simpljoin1.
+      clear H7.
+      eapply program_step_deterministic in H6; eauto.
+      simpljoin1.
+      eapply program_step_deterministic in H11; eauto.
+      simpljoin1.
+      exists fp fq L (r' ** r).
+      eapply disj_sep_star_merge with (p2 := r) in H12; eauto.
+      eapply sep_star_assoc2 in H12.
+      repeat (split; eauto).
+      intros.
+      eapply sep_star_assoc in H6.
+      eapply sep_star_subst; eauto.
+      simpl; eauto.
+      simpl; eauto.
     }
-    
 
-(*+ Instruction Sequence Rule Sound +*) 
+  - (** J2 *)
+    inversion H; subst.
+    renames l to pc, l0 to npc.
+    inversion H4; get_ins_diff_false.
+    eapply jmpl_seq; eauto.
+    simpljoin1.
+    {
+      clear H7.
+      eapply program_step_safety_property with (s := (m1 ⊎ m0, (r1 ⊎ r0, f0), d0)) in H6;
+        eauto.
+      simpljoin1.
+      destruct_state x.
+      destruct_state x6.
+      simpls.
+      simpljoin1.
+      eapply program_step_safety_property with (s := (m ⊎ m2, (r2 ⊎ r3, f1), d1)) in H8;
+        eauto.
+      simpljoin1.
+      destruct_state x0.
+      destruct_state x5.
+      simpls.
+      simpljoin1.
+      do 6 eexists.
+      eauto.
+      simpl; eauto.
+      simpl; eauto.
+    }
+    {
+      simpljoin1.
+      lets Hp : H6. 
+      eapply H7 with (S1 := x) in Hp; eauto.
+      simpljoin1.
+      renames x5 to fp, x6 to fq, x7 to L, x8 to r'.
+      clear H7. 
+      eapply program_step_safety_property with (s := (m1 ⊎ m0, (r1 ⊎ r0, f0), d0)) (r := r)
+        in H6; eauto.
+      simpljoin1.
+      destruct_state x.
+      destruct_state x6.
+      simpl in H7.
+      simpljoin1. 
+      eapply program_step_safety_property with (s := (m ⊎ m2, (r2 ⊎ r3, f1), d1)) (r := r)
+        in H8; eauto.
+      simpljoin1.
+      destruct_state x0.
+      destruct_state x5.
+      simpl in H16.
+      simpljoin1.
+      intros.
+      eapply program_step_deterministic in H6; eauto.
+      simpljoin1.
+      eapply program_step_deterministic in H8; eauto.
+      simpljoin1.
+      exists fp fq L (r' ** r).
+      repeat (split; eauto).
+      eapply disj_sep_star_merge with (p2 := r) in H9; eauto.
+      eapply sep_star_assoc2 in H9; eauto.
+      intros.
+      eapply sep_star_assoc in H6.
+      eapply sep_star_subst; eauto.
+      simpl; eauto.
+      simpl; eauto.
+    }
+
+  - (** call f *)
+    inversion H; subst.
+    renames l to pc.
+    inversion H4; get_ins_diff_false.
+    eapply call_seq; eauto.
+    {
+      clear H7.
+      simpljoin1.
+      eapply program_step_safety_property with (s := (m1 ⊎ m0, (r1 ⊎ r0, f0), d0)) in H6;
+        eauto.
+      simpljoin1.
+      destruct_state x.
+      destruct_state x6.
+      simpl in H6.
+      simpljoin1.
+      eapply program_step_safety_property with (s := (m ⊎ m2, (r2 ⊎ r3, f2), d1)) in H7;
+        eauto.
+      simpljoin1.
+      destruct_state x0.
+      destruct_state x5.
+      simpls.
+      simpljoin1.
+      do 6 eexists.
+      eauto.
+      simpl; eauto.
+      simpl; eauto.
+    }
+    {
+      simpljoin1.
+      lets Hp : H6.
+      eapply H7 with (S1 := x) in Hp; eauto.
+      clear H7.
+      simpljoin1; eauto.
+      renames x5 to fp, x6 to fq, x7 to L, x8 to r'.
+      eapply program_step_safety_property with (s := (m1 ⊎ m0, (r1 ⊎ r0, f0), d0)) (r := r)
+        in H6; eauto.
+      simpljoin1.
+      destruct_state x.
+      destruct_state x4.
+      simpl in H6.
+      simpljoin1.
+      eapply program_step_safety_property with (s := (m ⊎ m2, (r2 ⊎ r3, f2), d1)) (r := r)
+        in H8; eauto.
+      simpljoin1.
+      destruct_state x0.
+      destruct_state x3.
+      simpl in H18.
+      simpljoin1.
+      intros.
+      eapply program_step_deterministic in H5; eauto.
+      simpljoin1.
+      eapply program_step_deterministic in H8; eauto.
+      simpljoin1.
+      exists fp fq L (r' ** r).
+      repeat (split; eauto).
+      eapply disj_sep_star_merge with (p2 := r) in H10; eauto.
+      eapply sep_star_assoc2; eauto.
+      intros.
+      eapply sep_star_assoc in H5.
+      eapply sep_star_split in H5.
+      simpljoin1.
+      destruct_state x.
+      destruct_state x0.
+      simpl in H23.
+      simpljoin1.
+      eapply H13 in H5.
+      eapply IHI; eauto.
+      clear - H16.
+      do 2 rewrite Int.add_assoc in H16.
+      eauto.
+      simpl; eauto.
+      simpl; eauto.
+    }
+
+  - (** retl *)
+    inversion H; subst.
+    renames l to pc, l0 to npc.
+    inversion H4; subst; get_ins_diff_false.
+    clear H H5.
+    eapply ret_seq; eauto.
+    {
+      simpljoin1.
+      eapply program_step_safety_property with (s := (m1 ⊎ m0, (r1 ⊎ r0, f0), d0))
+        in H; eauto.
+      simpljoin1.
+      destruct_state x.
+      destruct_state x6.
+      simpl in H6.
+      simpljoin1.
+      eapply program_step_safety_property with (s := (m ⊎ m2, (r2 ⊎ r3, f1), d1))
+        in H5; eauto.
+      simpljoin1.
+      destruct_state x0.
+      destruct_state x5.
+      simpl in H11.
+      simpljoin1.
+      do 6 eexists.
+      eauto.
+      simpl; eauto.
+      simpl; eauto.
+    }
+    {
+      simpljoin1.
+      lets Hp : H.
+      eapply H7 with (S1 := x) in Hp; eauto.
+      simpljoin1.
+      clear H7.
+      eapply program_step_safety_property with
+      (s := (m1 ⊎ m0, (r1 ⊎ r0, f0), d0)) (r := r) in H; eauto.
+      simpljoin1.
+      destruct_state x.
+      destruct_state x4.
+      simpl in H7.
+      simpljoin1.
+      eapply program_step_safety_property with
+      (s := (m ⊎ m2, (r2 ⊎ r3, f1), d1)) (r := r) in H5; eauto.
+      simpljoin1.
+      destruct_state x0.
+      destruct_state x3.
+      simpl in H13.
+      simpljoin1.
+      simpls.
+      intros.
+      eapply program_step_deterministic in H; eauto.
+      simpljoin1.
+      eapply program_step_deterministic in H5; eauto.
+      simpljoin1.
+      split; eauto.
+      exists (m3, (r4, f2), d2) (m4, (r5, f2), d2).
+      simpl.
+      repeat (split; eauto).
+      exists x5.
+      split; eauto.
+      simpl.
+      unfold merge.
+      rewrite H8; eauto.
+      simpl; eauto.
+      simpl; eauto.
+    }
+
+  - (** be aexp *)
+    inversion H; subst.
+    renames l to pc, l0 to npc.
+    inversion H4; subst; get_ins_diff_false.
+    clear H H5.
+    eapply be_seq; eauto.
+    {
+      clear H7.
+      simpljoin1.
+      eapply program_step_safety_property with (s := (m1 ⊎ m0, (r1 ⊎ r0, f0), d0)) (r := r)
+        in H; eauto.
+      simpljoin1.
+      destruct_state x.
+      destruct_state x6.
+      simpls.
+      simpljoin1.
+      eapply program_step_safety_property with (s := (m ⊎ m2, (r2 ⊎ r3, f1), d1)) (r := r)
+        in H5; eauto.
+      simpljoin1.
+      do 6 eexists.
+      eauto.
+      simpl; eauto.
+      simpl; eauto.
+    }
+    {
+      simpljoin1.
+      lets Hp : H.
+      eapply H7 with (S1 := x) in H; eauto.
+      clear H7.
+      simpljoin1.
+      simpl in H.
+      eapply program_step_safety_property with (s := (m1 ⊎ m0, (r1 ⊎ r0, f0), d0)) (r := r)
+        in Hp; eauto.
+      simpljoin1.
+      destruct_state x.
+      destruct_state x7.
+      simpl in H9.
+      simpljoin1.
+      eapply program_step_safety_property with (s := (m ⊎ m2, (r2 ⊎ r3, f1), d1)) (r := r)
+        in H5; eauto.
+      simpljoin1.
+      destruct_state x0.
+      destruct_state x6.
+      simpl in H13.
+      simpljoin1.
+      intros.
+      eapply program_step_deterministic in H8; eauto.
+      simpljoin1.
+      eapply program_step_deterministic in H5; eauto.
+      simpljoin1.
+      exists x5.
+      split; eauto.
+      simpl.
+      unfold merge.
+      rewrite H; eauto.
+      split.
+      {
+        intros.
+        eapply H6 in H5.
+        simpljoin1.
+        renames x to fp, x0 to fq, x6 to L, x7 to r'.
+        exists fp fq L (r' ** r).
+        repeat (split; eauto).
+        eapply disj_sep_star_merge with (p2 := r) in H8; eauto.
+        eapply sep_star_assoc2; eauto.
+        intros.
+        eapply sep_star_assoc in H22.
+        eapply sep_star_subst; eauto.
+      }
+      {
+        intros.
+        lets Hfalse : H5.
+        eapply H7 in H5.
+        eapply IHI; eauto.
+        inversion H18; subst. 
+        inversion H33; get_ins_diff_false.
+        eapply regz_exe_delay_stable2 in H36; eauto.
+        clear - H H36 H37.
+        unfold merge in *.
+        rewrite H in H36; eauto.
+        inversion H36; subst.
+        tryfalse. 
+        inversion H19; subst. 
+        inversion H40; get_ins_diff_false.
+        clear - H15.
+        rewrite Int.add_assoc; eauto.
+      }
+
+      simpl; eauto.
+      simpl; eauto.
+    }
+
+  - (** bne aexp *)
+    inversion H; subst.
+    renames l to pc, l0 to npc.
+    inversion H4; subst; get_ins_diff_false.
+    clear H H5.
+    eapply bne_seq; eauto.
+    {
+      clear H7.
+      simpljoin1.
+      eapply program_step_safety_property with (s := (m1 ⊎ m0, (r1 ⊎ r0, f0), d0)) in H;
+        eauto.
+      simpljoin1.
+      destruct_state x.
+      destruct_state x6.
+      simpl in H6.
+      simpljoin1.
+      eapply program_step_safety_property with (s := (m ⊎ m2, (r2 ⊎ r3, f1), d1)) in H5;
+        eauto.
+      simpljoin1.
+      do 6 eexists.
+      eauto.
+      simpl; eauto.
+      simpl; eauto.
+    }
+    {
+      simpljoin1.
+      lets Hp : H.
+      eapply H7 with (S1 := x) in Hp; eauto.
+      clear H7.
+      eapply program_step_safety_property with (s := (m1 ⊎ m0, (r1 ⊎ r0, f0), d0)) in H;
+        eauto.
+      simpljoin1.
+      destruct_state x.
+      destruct_state x6.
+      simpl in H7.
+      simpljoin1.
+      simpl in H6.
+      eapply program_step_safety_property with (s := (m ⊎ m2, (r2 ⊎ r3, f1), d1)) in H5;
+        eauto.
+      simpljoin1.
+      destruct_state x0.
+      destruct_state x5.
+      simpl in H13.
+      simpljoin1.
+      intros.
+      eapply program_step_deterministic in H; eauto.
+      simpljoin1.
+      eapply program_step_deterministic in H5; eauto.
+      simpljoin1.
+      exists x7.
+      repeat (split; eauto).
+      simpl.
+      unfold merge.
+      rewrite H6; eauto.
+      intros.
+      eapply H9 in H.
+      simpljoin1.
+      renames x to fp, x0 to fq, x5 to L, x6 to r'.
+      exists fp fq L (r' ** r).
+      repeat (split; eauto).
+      eapply disj_sep_star_merge with (p2 := r) in H5; eauto.
+      eapply sep_star_assoc2; eauto.
+      intros.
+      eapply sep_star_assoc in H22.
+      eapply sep_star_subst; eauto.
+
+      intros.
+      lets Hfalse : H.
+      eapply H10 in H.
+      eapply IHI; eauto.
+      inversion H18; subst.
+      inversion H33; get_ins_diff_false; subst.
+      eapply regz_exe_delay_stable2 in H36; eauto.
+      unfold merge in H36.
+      rewrite H6 in H36.
+      inversion H36; subst.
+      tryfalse.
+      inversion H19; subst.
+      inversion H41; get_ins_diff_false.
+      clear - H15.
+      rewrite Int.add_assoc; eauto.
+
+      simpl; eauto.
+      simpl; eauto.
+    }
+Qed.
+    
+(*+ Instruction Sequence Rule Sound +*)
+Theorem wf_seq_seq_rule :
+  forall p p' i q f Spec I,
+    ins_sound (p ↓) p' i -> insSeq_sound Spec p' I q ->
+    insSeq_sound Spec p (f#i;;I) q.
+Proof.
+  intros.
+  unfolds insSeq_sound.
+  intros.
+  inversion H1; subst.
+  unfolds ins_sound.
+  eapply i_seq; eauto.
+
+  (** progress *)
+  destruct_state S.
+  assert (exists R' D', exe_delay r d = (R', D')).
+  {    
+    eapply exe_delay_no_abort; eauto.
+  }
+  simpljoin1.
+  renames x to R', x0 to D'.
+  lets Hexe_delay : H3.
+  symmetry in H3.
+  eapply dly_reduce_asrt_stable in H3; eauto.
+  eapply H in H3; eauto.
+  simpljoin1.
+  exists x npc (npc +ᵢ ($ 4)).
+  destruct_state x.
+  econstructor; eauto.
+  eapply NTrans; eauto.
+
+  (** preservation *)
+  intros.
+  inversion H3; subst.
+  eapply dly_reduce_asrt_stable in H7; eauto.
+  eapply H in H7; eauto.
+  simpljoin1.
+  inversion H14; get_ins_diff_false.
+  eapply ins_exec_deterministic in H4; eauto.
+  simpljoin1.
+  eapply H0 in H5; eauto.
+Qed.
+
+Theorem wf_seq_call_rule :
+  forall p q fp fq L f p1 p2 p' v i Spec r I f1 f2,
+    Spec (f, f +ᵢ ($ 4)) = Some (fp, fq) ->
+    (p ↓) ==> r15 |=> v ** p1 -> ins_sound (r15 |=> f1 ** p1 ↓) p2 i ->
+    fp L ==> Or r15 ==ₑ f1 -> p2 ==> fp L ** r ->
+    fq L ** r ==> p' -> fq L ==> Or r15 ==ₑ f1 -> DlyFrameFree r ->
+    insSeq_sound Spec p' I q ->
+    insSeq_sound Spec p (f1 c> call f;; f2 c> i;;I) q.
+Proof.
+  intros.
+  unfold insSeq_sound.
+  intros.
+  inversion H8; subst.
+  eapply call_seq; eauto.
+
+  (** progress *)
+  destruct_state S.
+  assert (exists R' D', exe_delay r0 d = (R', D')).
+  {    
+    eapply exe_delay_no_abort; eauto.
+  }
+  simpljoin1.
+  renames x to R', x0 to D'.
+  lets Hexe_delay : H10.
+  symmetry in Hexe_delay.
+  eapply dly_reduce_asrt_stable in Hexe_delay; eauto.
+  eapply H0 in Hexe_delay.
+  lets Hf : Hexe_delay.
+  eapply reg_vl_change with (v1 := f1) in Hf; eauto.
+  assert (exists R'' D'', exe_delay (set_R R' r15 f1) D' = (R'', D'')).
+  {    
+    eapply exe_delay_no_abort; eauto.
+  }
+  simpljoin1.
+  lets Hexe_delay2 : H11.
+  renames x to R'', x0 to D''.
+  symmetry in H11.
+  eapply dly_reduce_asrt_stable in H11; eauto.
+  eapply H1 in H11; eauto.
+  simpljoin1.
+  exists (m, (set_R R' r15 f1, f0), D') x (f1 +ᵢ ($ 4)) f f (f +ᵢ ($ 4)).
+  split; eauto.
+  econstructor; eauto.
+  eapply Call; eauto.
+  clear - Hexe_delay.
+  sep_star_split_tac.
+  simpls.
+  simpljoin1.
+  unfolds regSt.
+  simpls.
+  simpljoin1.
+  eapply indom_merge_still; eauto.
+  eapply regset_l_l_indom; eauto.
+  destruct_state x.
+  econstructor; eauto.
+  eapply NTrans; eauto.
+
+  (** preservation *)
+  intros.
+  inversion H10; subst.
+  inversion H23; get_ins_diff_false.
+  clear H18.
+  inversion H11; subst. 
+  inversion H28; get_ins_diff_false.
+  exists fp fq L r.
+  repeat (split; eauto).
+  eapply dly_reduce_asrt_stable in H15; eauto.
+  eapply H0 in H15.
+  eapply reg_vl_change with (v1 := f1) in H15; eauto.
+  eapply dly_reduce_asrt_stable in H16; eauto.
+  eapply H1 in H16.
+  simpljoin1.
+  eapply ins_exec_deterministic in H26; eauto.
+  simpljoin1.
+  eauto.
+  intros.
+  eapply H4 in H12.
+  clear - H7 H21 H12.
+  unfolds insSeq_sound.
+  eapply H7 in H21; eauto.
+  do 2 rewrite Int.add_assoc in H21; eauto.
+  eapply H2 in H12.
+  clear - H12.
+  destruct_state S'.
+  simpls.
+  eauto.
+  eapply H5 in H13.
+  clear - H13.
+  destruct_state S''.
+  simpls.
+  eauto.
+Qed.
+
+Theorem wf_seq_ret_rule :
+  forall p p' q i Spec f1 f2,
+    ins_sound ((p ↓) ↓) p' i ->
+    p' ==> q -> fretSta ((p ↓) ↓) p' ->
+    insSeq_sound Spec p (f1 r> retl ;; f2 r> i) q.
+Proof.
+  intros.
+  unfolds insSeq_sound.
+  intros.
+  inversion H2; subst.
+  eapply ret_seq; eauto.
+
+  (** progress *)
+  destruct_state S.
+  assert (exists R' D', exe_delay r d = (R', D')).
+  {
+    eapply exe_delay_no_abort; eauto.
+  }
+  simpljoin1.
+  renames x to R', x0 to D'.
+  symmetry in H4.
+  lets Hexe_delay1 : H4.
+  eapply dly_reduce_asrt_stable in Hexe_delay1; eauto.
+  assert (exists R'' D'', exe_delay R' D' = (R'', D'')).
+  {
+    eapply exe_delay_no_abort; eauto.
+  }
+  simpljoin1.
+  renames x to R'', x0 to D''.
+  symmetry in H5.
+  lets Hexe_delay2 : H5. 
+  eapply dly_reduce_asrt_stable in Hexe_delay2; eauto.
+  lets Hp' : Hexe_delay2.
+  eapply H in Hp'; eauto.
+  simpljoin1.
+  lets Hret_f : H7.
+  eapply H1 in Hret_f; eauto.
+  simpljoin1. 
+  exists (m, (R', f), D') x f2 (x0 +ᵢ ($ 8)) (x0 +ᵢ ($ 8)) ((x0 +ᵢ ($ 8)) +ᵢ ($ 4)).
+  split; eauto.
+  econstructor; eauto.
+  eapply Retl; eauto.
+  simpls.
+  clear - H5 H8.
+  eapply exe_delay_general_reg_stable; eauto.
+  destruct_state x.
+  econstructor; eauto.
+  eapply NTrans; eauto.
+
+  (** preservation *)
+  intros.
+  inversion H4; subst.
+  inversion H16; get_ins_diff_false.
+  clear H12.
+  inversion H5; subst.
+  inversion H21; get_ins_diff_false.
+  lets Hexe_delay1 : H10.
+  lets Hexe_delay2 : H12.
+  eapply dly_reduce_asrt_stable in H10; eauto.
+  eapply dly_reduce_asrt_stable in H12; eauto.
+  lets Hp' : H12.
+  eapply H in Hp'; eauto.
+  simpljoin1. 
+  eapply ins_exec_deterministic in H19; eauto.
+  subst.
+  split; eauto.
+  exists f.
+  simpl.
+  repeat (split; eauto).
+  eapply H1 in H7; eauto.
+  simpljoin1.
+  simpls.
+  symmetry in Hexe_delay2.
+  eapply exe_delay_general_reg_stable with (r := r15) in Hexe_delay2; eauto.
+  eapply Hexe_delay2 in H24.
+  rewrite H24 in H7.
+  inversion H7; subst.
+  eauto.
+  rewrite Int.add_assoc; eauto.
+Qed.
+
+Theorem wf_seq_j1_rule :
+  forall f1 f2 f aexp (r1 : GenReg) i p p' p1 q fp fq r Spec L v,
+    Spec (f, f +ᵢ ($ 4)) = Some (fp, fq) ->
+    (p ↓) ==> aexp ==ₓ f -> (p ↓) ==> r1 |=> v ** p1 ->
+    ins_sound (r1 |=> f1 ** p1 ↓) p' i ->
+    p' ==> fp L ** r -> fq L ** r ==> q -> DlyFrameFree r ->
+    insSeq_sound Spec p (consJ1 f1 aexp r1 f2 i) q.
+Proof.
+  intros.
+  unfold insSeq_sound.
+  intros.
+  inversion H6; subst.
+  eapply jmpl_seq; eauto.
+
+  (** progress *)
+  destruct_state S.
+  assert (exists R' D', exe_delay r0 d = (R', D')).
+  {
+    eapply exe_delay_no_abort; eauto.
+  }
+  simpljoin1.
+  renames x to R', x0 to D'.
+  lets Hexe_delay1 : H8.
+  symmetry in Hexe_delay1.
+  eapply dly_reduce_asrt_stable in Hexe_delay1; eauto.
+  lets Haexp : Hexe_delay1.
+  lets Hf1 : Hexe_delay1.
+  eapply H0 in Haexp.
+  eapply H1 in Hf1.
+  lets Hf1' : Hf1.
+  eapply reg_vl_change with (v1 := f1) in Hf1'; eauto.
+  assert (exists R'' D'', exe_delay (set_R R' r1 f1) D' = (R'', D'')).
+  {
+    eapply exe_delay_no_abort; eauto.
+  }
+  simpljoin1.
+  renames x to R'', x0 to D''.
+  lets Hexe_delay2 : H9.
+  symmetry in Hexe_delay2.
+  eapply dly_reduce_asrt_stable in Hexe_delay2; eauto.
+  eapply H2 in Hexe_delay2; eauto.
+  simpljoin1. 
+  exists (m, (set_R R' r1 f1, f0), D') x f2 f f (f +ᵢ ($ 4)).
+  split; eauto.
+  econstructor; eauto.
+  eapply Jumpl; eauto.
+  clear - Haexp.
+  simpls; eauto.
+  simpljoin1; eauto.
+  clear - Haexp.
+  simpls.
+  simpljoin1; eauto.
+  clear - Hf1.
+  sep_star_split_tac.
+  simpls.
+  simpljoin1.
+  unfolds regSt.
+  simpls.
+  simpljoin1.
+  eapply indom_merge_still; eauto.
+  eapply regset_l_l_indom; eauto.
+  destruct_state x.
+  econstructor; eauto.
+  eapply NTrans; eauto.
+
+  (** preservation *)
+  intros.
+  inversion H8; subst.
+  eapply dly_reduce_asrt_stable in H14; eauto.
+  lets Haexp : H14.
+  lets Hf1 : H14.
+  eapply H0 in Haexp.
+  simpl in Haexp.
+  simpljoin1.
+  inversion H20; get_ins_diff_false.
+  rewrite H10 in H30.
+  inversion H30; subst.
+  clear H30.
+  inversion H9; subst. 
+  inversion H28; get_ins_diff_false.
+  exists fp fq L r.
+  repeat (split; eauto).
+  eapply H1 in Hf1.
+  eapply reg_vl_change with (v1 := f1) in Hf1; eauto.
+  eapply dly_reduce_asrt_stable in H18; eauto.
+  eapply H2 in H18; eauto.
+  simpljoin1.
+  eapply ins_exec_deterministic in H26; eauto.
+  subst.
+  eauto.
+Qed.
+
+Theorem wf_seq_J2_rule :
+  forall p p1 p2 q f1 f1' f2 f2' aexp1 aexp2 (r1 r2 : GenReg) fp fq L r Spec v1 v2,
+    Spec (f1', f2') = Some (fp, fq) ->
+    (p ↓) ==> aexp1 ==ₓ f1' -> (p ↓) ==> r1 |=> v1 ** p1 ->
+    (r1 |=> f1 ** p1 ↓) ==> aexp2 ==ₓ f2' -> (r1 |=> f1 ** p1 ↓) ==> r2 |=> v2 ** p2 ->
+    r2 |=> f2 ** p2 ==> fp L ** r -> fq L ** r ==> q -> DlyFrameFree r ->
+    insSeq_sound Spec p (consJ2 f1 aexp1 r1 f2 aexp2 r2) q.
+Proof.
+  intros.
+  unfold insSeq_sound.
+  intros.
+  inversion H7; subst.
+  eapply jmpl_seq; eauto.
+
+  (** progress *)
+  destruct_state S.
+  assert (exists R' D', exe_delay r0 d = (R', D')).
+  {
+    eapply exe_delay_no_abort; eauto.
+  }
+  simpljoin1.
+  renames x to R', x0 to D'.
+  lets Hexe_delay1 : H9.
+  symmetry in Hexe_delay1.
+  eapply dly_reduce_asrt_stable in Hexe_delay1; eauto.
+  lets Haexp1 : Hexe_delay1.
+  lets Hf1 : Hexe_delay1.
+  eapply H0 in Haexp1.
+  eapply H1 in Hf1.
+  lets Hf1' : Hf1.
+  eapply reg_vl_change with (v1 := f1) in Hf1; eauto.
+  assert (exists R'' D'', exe_delay (set_R R' r1 f1) D' = (R'', D'')).
+  {
+    eapply exe_delay_no_abort; eauto.
+  }
+  simpljoin1.
+  renames x to R'', x0 to D''.
+  lets Hexe_delay2 : H10.
+  symmetry in Hexe_delay2.
+  eapply dly_reduce_asrt_stable in Hexe_delay2; eauto.
+  lets Haexp2 : Hexe_delay2.
+  lets Hf2 : Hexe_delay2.
+  eapply H2 in Haexp2; eauto.
+  eapply H3 in Hf2; eauto.
+  simpl in Haexp1.
+  simpl in Haexp2.
+  simpljoin1.
+  exists (m, (set_R R' r1 f1, f), D') (m, (set_R R'' r2 f2, f), D'') f2 f1' f1' f2'.
+  split; eauto.
+  econstructor; eauto.
+  eapply Jumpl; eauto.
+  clear - Hf1'.
+  sep_star_split_tac.
+  simpls.
+  unfolds regSt.
+  simpls.
+  simpljoin1.
+  eapply indom_merge_still; eauto.
+  eapply regset_l_l_indom; eauto.
+  econstructor; eauto.
+  eapply Jumpl; eauto.
+  clear - Hf2.
+  sep_star_split_tac.
+  simpls.
+  unfolds regSt.
+  simpls.
+  simpljoin1.
+  eapply indom_merge_still; eauto.
+  eapply regset_l_l_indom; eauto.
+
+  (** preservation *)
+  intros.
+  inversion H9; subst.
+  eapply dly_reduce_asrt_stable in H15; eauto.
+  lets Haexp1 : H15.
+  lets Hf1 : H15.
+  eapply H0 in Haexp1.
+  eapply H1 in Hf1.
+  inversion H21; get_ins_diff_false.
+  simpl in Haexp1.
+  simpljoin1.
+  rewrite H11 in H29.
+  inversion H29; subst.
+  clear H29.
+  inversion H10; subst.
+  lets Hf1' : Hf1.
+  eapply reg_vl_change with (v1 := f1) in Hf1'; eauto.
+  eapply dly_reduce_asrt_stable in H18; eauto.
+  lets Haexp2 : H18.
+  lets Hf2 : H18.
+  eapply H2 in Haexp2.
+  eapply H3 in Hf2.
+  simpl in Haexp2.
+  simpljoin1.
+  inversion H28; get_ins_diff_false.
+  rewrite H13 in H37.
+  inversion H37; subst.
+  exists fp fq L r.
+  repeat (split; eauto).
+  eapply reg_vl_change with (v1 := pc1) in Hf2; eauto.
+Qed.
+
+Lemma wf_seq_be_rule :
+  forall p p' q r f1 f2 f aexp i fp fq L I bv Spec,
+    Spec (f, f +ᵢ ($ 4)) = Some (fp, fq) -> DlyFrameFree r ->
+    (p ↓) ==> aexp ==ₓ f -> (p ↓) ==> z |=> bv ** Atrue ->
+    ins_sound ((p ↓) ↓) p' i ->
+    (bv =ᵢ ($ 0) = false -> p' ==> fp L ** r /\ fq L ** r ==> q) ->
+    insSeq_sound Spec (p' //\\ [|bv =ᵢ ($ 0) = true|]) I q ->
+    insSeq_sound Spec p (f1 e> be aexp;; f2 e> i;;I) q.
+Proof.
+  introv H Hr.
+  intros.
+  unfold insSeq_sound.
+  intros.
+  inversion H5; subst.
+  eapply be_seq; eauto.
+
+  (** progress *)
+  destruct_state S.
+  assert (exists R' D', exe_delay r0 d = (R', D')).
+  {
+    eapply exe_delay_no_abort; eauto.
+  }
+  simpljoin1.
+  renames x to R', x0 to D'.
+  lets Hp : H7.
+  symmetry in Hp.
+  eapply dly_reduce_asrt_stable in Hp; eauto.
+  assert (exists R'' D'', exe_delay R' D' = (R'', D'')).
+  {
+    eapply exe_delay_no_abort; eauto.
+  }
+  simpljoin1.
+  renames x to R'', x0 to D''.
+  lets Hp' : H8.
+  symmetry in Hp'.
+  eapply dly_reduce_asrt_stable in Hp'; eauto.
+  eapply H2 in Hp'.
+  simpljoin1.
+  lets Hz : Hp.
+  eapply H1 in Hz.
+  destruct (Int.eq bv ($ 0)) eqn:Heqe.
+  {
+    exists (m, (R', f0), D') x f2 (f2 +ᵢ ($ 4)) (f2 +ᵢ ($ 4)) ((f2 +ᵢ ($ 4)) +ᵢ ($ 4)).
+    split; eauto.
+    econstructor; eauto.
+    eapply Be_false with (f := f); eauto.
+    eapply H0 in Hp.
+    clear - Hp.
+    simpls.
+    simpljoin1; eauto.
+    clear - Heqe Hz.
+    sep_star_split_tac.
+    simpls.
+    simpljoin1.
+    unfolds regSt.
+    simpls.
+    simpljoin1.
+    eapply int_eq_true_eq in Heqe.
+    unfold merge.
+    subst.
+    unfold RegMap.set.
+    destruct_rneq; eauto.
+    eapply H0 in Hp.
+    clear - Hp.
+    simpls.
+    simpljoin1; eauto.
+    destruct_state x.
+    econstructor; eauto.
+    eapply NTrans; eauto.
+  }
+  { 
+    exists (m, (R', f0), D') x f2 f f (f +ᵢ ($ 4)).
+    split; eauto.
+    econstructor; eauto.
+    eapply Be_true with (v := bv); eauto.
+    eapply H0 in Hp.
+    clear - Hp.
+    simpls.
+    simpljoin1; eauto.
+    clear - Hz.
+    sep_star_split_tac.
+    simpls.
+    unfolds regSt.
+    simpls.
+    simpljoin1.
+    unfold merge.
+    unfold RegMap.set.
+    destruct_rneq.
+    clear - Heqe.
+    eapply int_eq_false_neq in Heqe; eauto.
+    eapply H0 in Hp.
+    clear - Hp.
+    simpls.
+    simpljoin1; eauto.
+    destruct_state x.
+    econstructor; eauto.
+    eapply NTrans; eauto.
+  }
+
+  (** preservation *)
+  intros.
+  inversion H7; subst.
+  inversion H8; subst.
+  exists bv.
+  split; eauto.
+  lets Hexe_delay1 : H12.
+  eapply dly_reduce_asrt_stable in H12; eauto.
+  inversion H20; get_ins_diff_false.
+  eapply dly_reduce_asrt_stable in H14; eauto.
+  clear H21. 
+  eapply H1 in H12.  
+  clear - Hexe_delay1 H12 H31.
+  sep_star_split_tac.
+  simpls. 
+  unfolds regSt.
+  simpls. 
+  simpljoin1.
+  lets Hz : H31.
+  unfold merge in Hz.
+  unfold RegMap.set in Hz.
+  destruct_rneq_H.
+  inversion Hz; subst.
+  eapply regz_exe_delay_stable2; eauto.
+  simpl.
+  eapply H1 in H12.
+  clear - Hexe_delay1 H12 H31.
+  sep_star_split_tac.
+  simpls.
+  unfolds regSt.
+  simpls.
+  simpljoin1.
+  lets Hz : H31.
+  unfold RegMap.set in Hz.
+  unfold merge in Hz.
+  destruct_rneq_H.
+  inversion Hz; subst.
+  eapply regz_exe_delay_stable2; eauto.
+  split.
+  {
+    intros.
+    eapply dly_reduce_asrt_stable in H12; eauto.
+    lets Hz : H12.
+    eapply H1 in Hz.
+    inversion H20; get_ins_diff_false.
+    inversion H25; get_ins_diff_false.
+    exists fp fq L r.
+    lets Hp : H12.
+    eapply H0 in H12.
+    simpl in H12.
+    simpljoin1.
+    rewrite H10 in H31.
+    inversion H31; subst. 
+    split; eauto.
+    eapply dly_reduce_asrt_stable in Hp; eauto.
+    eapply H2 in Hp; eauto.
+    simpljoin1. 
+    eapply ins_exec_deterministic in H26; eauto.
+    subst.
+    assert (bv = v).
+    {
+      clear - Hz H32.
+      sep_star_split_tac.
+      simpls.
+      unfolds regSt.
+      simpls.
+      simpljoin1.
+      unfold merge in *.
+      unfolds RegMap.set.
+      destruct_rneq_H.
+      inversion H32; subst.
+      eauto.
+    }
+    subst.
+    assert (v =ᵢ ($ 0) = false).
+    {
+      unfold Int.eq.
+      clear - H33.
+      destruct (zeq (Int.unsigned v) (Int.unsigned $ 0)) eqn:Heqe; eauto.
+      clear Heqe.
+      eapply z_eq_to_int_eq in e; eauto.
+      do 2 rewrite Int.repr_unsigned in e; eauto.
+      subst.
+      tryfalse.
+    }
+    eapply H3 in H18; eauto.
+    simpljoin1.
+    repeat (split; eauto).
+    assert (bv = $ 0).
+    {
+      clear - Hz H32.
+      sep_star_split_tac.
+      simpls.
+      unfolds regSt.
+      simpls.
+      simpljoin1.
+      unfold merge in *.
+      unfolds RegMap.set.
+      destruct_rneq_H.
+      inversion H32; eauto.
+    }
+    subst.
+    tryfalse.
+  }
+  {
+    intros. 
+    eapply dly_reduce_asrt_stable in H12; eauto.
+    inversion H20; get_ins_diff_false.
+    eapply H1 in H12. 
+    clear - H12 H32 H33.
+    sep_star_split_tac.
+    simpls.
+    unfolds regSt.
+    simpls. 
+    simpljoin1.
+    unfold merge in *.
+    unfolds RegMap.set.
+    destruct_rneq_H.
+    inversion H32; subst.
+    eapply dly_reduce_asrt_stable in H14; eauto.
+    eapply H2 in H14.
+    simpljoin1.
+    inversion H25; get_ins_diff_false.
+    eapply ins_exec_deterministic in H9; eauto.
+    subst.  
+    clear - H4 H17 H10 H11.
+    unfolds insSeq_sound.
+    eapply H4; eauto.
+    rewrite Int.add_assoc; eauto.
+    simpl.
+    split; eauto.
+  }
+Qed.
+
+Lemma wf_seq_bne_rule :
+  forall p p' q r f1 f2 f aexp i fp fq L I bv Spec,
+    Spec (f, f +ᵢ ($ 4)) = Some (fp, fq) -> DlyFrameFree r ->
+    (p ↓) ==> aexp ==ₓ f -> (p ↓) ==> z |=> bv ** Atrue ->
+    ins_sound ((p ↓) ↓) p' i ->
+    (bv =ᵢ ($ 0) = true -> p' ==> fp L ** r /\ fq L ** r ==> q) ->
+    insSeq_sound Spec (p' //\\ [|bv =ᵢ ($ 0) = false|]) I q ->
+    insSeq_sound Spec p (f1 n> bne aexp;; f2 n> i;;I) q.
+Proof.
+  introv H Hr.
+  intros.
+  unfold insSeq_sound.
+  intros.
+  inversion H5; subst.
+  eapply bne_seq; eauto.
+ 
+  (** progress *)
+  destruct_state S.
+  assert (exists R' D', exe_delay r0 d = (R', D')).
+  {
+    eapply exe_delay_no_abort; eauto.
+  }
+  simpljoin1.
+  renames x to R', x0 to D'.
+  lets Hp : H7.
+  symmetry in Hp.
+  eapply dly_reduce_asrt_stable in Hp; eauto.
+  assert (exists R'' D'', exe_delay R' D' = (R'', D'')).
+  {
+    eapply exe_delay_no_abort; eauto.
+  }
+  simpljoin1.
+  renames x to R'', x0 to D''.
+  lets Hp' : H8.
+  symmetry in Hp'.
+  eapply dly_reduce_asrt_stable in Hp'; eauto.
+  eapply H2 in Hp'.
+  simpljoin1.
+  lets Hz : Hp.
+  eapply H1 in Hz.
+  destruct (Int.eq bv ($ 0)) eqn:Heqe.
+  {
+    exists (m, (R', f0), D') x f2 f f (f +ᵢ ($ 4)).
+    split; eauto. 
+    econstructor; eauto.
+    eapply Bne_true; eauto.
+    eapply H0 in Hp.
+    clear - Hp.
+    simpls. 
+    simpljoin1; eauto.
+    clear - Hz Heqe.
+    sep_star_split_tac.
+    simpls.
+    unfolds regSt.
+    simpls.
+    simpljoin1.
+    unfold merge.
+    unfold RegMap.set.
+    destruct_rneq.
+    eapply int_eq_true_eq in Heqe; eauto.
+    subst; eauto.
+    eapply H0 in Hp.
+    simpl in Hp.
+    simpljoin1; eauto.
+    destruct_state x.
+    econstructor; eauto.
+    eapply NTrans; eauto.
+  }
+  {  
+    exists (m, (R', f0), D') x f2 (f2 +ᵢ ($ 4)) (f2 +ᵢ ($ 4)) ((f2 +ᵢ ($ 4)) +ᵢ ($ 4)).
+    split; eauto.
+    econstructor; eauto. 
+    eapply Bne_false with (v := bv) (f := f); eauto.
+    eapply H0 in Hp.
+    clear - Hp.
+    simpls.
+    simpljoin1; eauto.
+    clear - Heqe Hz.
+    sep_star_split_tac.
+    simpls.
+    simpljoin1.
+    unfolds regSt.
+    simpls.
+    simpljoin1.
+    unfold merge.
+    unfold RegMap.set.
+    destruct_rneq.
+    clear - Heqe. 
+    eapply int_eq_false_neq in Heqe; eauto.
+    eapply H0 in Hp.
+    simpls.
+    simpljoin1; eauto.
+    destruct_state x.
+    econstructor; eauto.
+    eapply NTrans; eauto.
+  }
+
+  (** preservation *)
+  intros.
+  inversion H7; subst.
+  inversion H8; subst. 
+  exists bv.
+  split; eauto. 
+  lets Hexe_delay1 : H12. 
+  eapply dly_reduce_asrt_stable in H12; eauto.
+  inversion H20; get_ins_diff_false.
+  eapply dly_reduce_asrt_stable in H14; eauto. 
+  eapply H1 in H12.   
+  clear - Hexe_delay1 H12 H31.
+  sep_star_split_tac.
+  simpls. 
+  unfolds regSt.
+  simpls. 
+  simpljoin1.
+  lets Hz : H31.
+  unfold merge in Hz.
+  unfold RegMap.set in Hz.
+  destruct_rneq_H.
+  inversion Hz; subst.
+  eapply regz_exe_delay_stable2; eauto.
+  simpl.
+  eapply H1 in H12.
+  clear - Hexe_delay1 H12 H31.
+  sep_star_split_tac.
+  simpls.
+  unfolds regSt.
+  simpls.
+  simpljoin1.
+  lets Hz : H31.
+  unfold RegMap.set in Hz.
+  unfold merge in Hz.
+  destruct_rneq_H.
+  inversion Hz; subst. 
+  eapply regz_exe_delay_stable2; eauto.
+  split.
+  {
+    intros.  
+    eapply dly_reduce_asrt_stable in H12; eauto.
+    lets Hp : H12.
+    inversion H20; get_ins_diff_false.
+    eapply H1 in H12. 
+    exists fp fq L r.
+    lets Haexp : Hp.
+    eapply H0 in Haexp.
+    simpl in Haexp.
+    simpljoin1.
+    rewrite H31 in H9.
+    inversion H9; subst.
+    clear H33.
+    inversion H25; get_ins_diff_false.
+    split; eauto.
+    eapply dly_reduce_asrt_stable in H14; eauto.
+    eapply H2 in H14; eauto.
+    simpljoin1.
+    eapply ins_exec_deterministic in H26; eauto.
+    subst.
+    assert (($ 0) =ᵢ ($ 0) = true).
+    eauto.
+    eapply H3 in H15.
+    simpljoin1.
+    repeat (split; eauto).
+    
+  }
+  {
+    
+  }
+Qed.
+  
 Theorem wf_seq_frame_rule :
   forall p q r I Spec,
     insSeq_sound Spec p I q -> DlyFrameFree r ->
@@ -308,6 +1611,8 @@ Proof.
   simpl in H6.
   simpljoin1.
   eapply H in H2; eauto.
+  eapply safety_ins_seq_frame_property; eauto.
+Qed.
 
 Theorem wf_seq_conseq_rule :
   forall I p p1 q1 q Spec,
@@ -322,6 +1627,21 @@ Proof.
   eapply safety_ins_seq_post_weak; eauto.
 Qed.
 
+Theorem wf_seq_ex_intro_rule :
+  forall tp (p : tp -> asrt) I q Spec,
+    (forall x' : tp, insSeq_sound Spec (p x') I q) ->
+    insSeq_sound Spec (EX x : tp, p x) I q.
+Proof.
+  intros.
+  unfold insSeq_sound.
+  intros.
+  simpls.
+  simpljoin1.
+  specialize (H x).
+  unfolds insSeq_sound.
+  eauto.
+Qed.
+  
 Theorem wf_seq_sound :
   forall Spec p q I,
     wf_seq Spec p I q ->
@@ -329,5 +1649,32 @@ Theorem wf_seq_sound :
 Proof.
   intros.
   induction H; intros.
-  Focus 10.
-Admitted.
+
+  -
+    eapply ins_rule_sound in H.
+    eapply wf_seq_seq_rule; eauto.
+
+  -
+    eapply ins_rule_sound in H1.
+    eapply wf_seq_call_rule; eauto.
+
+  -
+    eapply ins_rule_sound in H.
+    eapply wf_seq_ret_rule; eauto.
+
+  -
+    eapply ins_rule_sound in H2.
+    eapply wf_seq_j1_rule; eauto.
+
+  -
+    eapply wf_seq_J2_rule; eauto.
+
+  -
+    eapply ins_rule_sound in H1.
+    eapply wf_seq_be_rule; eauto.
+
+  -
+    eapply ins_rule_sound in H1.
+    
+
+>>>>>>>>>>>>>>>>>>>>>>>
